from [[1.1 Sets]]
## Theorem 1.1 De Morgan's Laws
Given n subsets $A_1,...,A_n$ of a universal set $U$, it can be said that
$$
( \bigcap\limits_{j=1}^{n} A_{j})^c = \bigcup\limits_{j=1}^{n} A_{j}^c \space\space \text{ or } \space\space (A \cap B)^c = A^c \cup B^c
$$
$$
( \bigcup\limits_{j=1}^{n} A_{j})^c = \bigcap\limits_{j=1}^{n} A_{j}^c \space\space \text{ or } \space\space (A \cup B)^c = A^c \cap B^c
$$

from [[1.2 Functions]]
## Theorem 1.2 properties of pre-images
Suppose $f \text{ : } A \rightarrow B$ is a function. suppose also that there is a set $S$ such that $S \subseteq A$.  a set $T$ such that $T \subseteq B$ and a set $T_i$ such that $T_i \subseteq B$ for every $i \in I$, where $I$ is a non-empty set. Then:
$$
S \subseteq f^{-1}(f(S)), \text{ and } f(f^{-1}(T)) \subseteq T
$$
$$
f^{-1}(\bigcup\limits_{i \in I} T_i) = \bigcup\limits_{i \in I} f^{-1}(T_i)
$$
$$
f^{-1}(\bigcap\limits_{i \in I} T_1) = \bigcap\limits_{i \in I} f^{-1}(T_1)
$$

