![video](https://www.youtube.com/watch?v=lwQG_dMXQOA&list=PLciPFwfwQdT9QD6P62J6xBbrs2yJFP3RF&index=1&ab_channel=MathCoursesbyDr.Ebrahimian)
### Notations
- Functions: $f:A \rightarrow B$ with a rule '$x$'  or $f$ is a function with domain $A$ and codomain $B$ that follows a rule $x$.
	- The domain $A$ ($D_f$ for a function $f$) are the 'allowed' **inputs** of a function
	- The codomain $B$ ($CO_f$ for a function $f$) are the 'allowed' **outputs** of a function
	- The range $R_f$ (or $\text{lm } f$) of a function $f$ are the 'actual' outputs of the function. It is defined as: $R_f = \{f(a) \text{ | } a \in D_f\}$ i.e. the values $f(a)$, where $a$ is an arbitrary element within $D_f$
*note that I invented the symbols used for domain and codomain and idk if they are actually used*
## 1.7 Functions
Given two non-empty sets $A$ and $B$, a function (or a mapping) $f: A \rightarrow B$ is a 'rule' that assigns every element $a \in A$ to an element $f(a) \in B$.

- The domain $A$ ($D_f$ for a function $f$) are the 'allowed' **inputs** of a function

- The codomain $B$ ($CO_f$ for a function $f$) are the 'allowed' **outputs** of a function

- The range $R_f$ (or $\text{lm } f$) of a function $f$ are the 'actual' outputs of the function. It if defined as: $R_f = \{f(a) \text{ | } a \in D_f\}$ i.e. the values $f(a)$, where $a$ is an arbitrary element within $D_f$
### Surjectivity
A function $f$ is surjective (or onto) $\iff$ for every element within its codomain $CO_f$ there is an element within its domain $D_f$ such that $f(a) = b$ 
- i.e. every element in $B$ is 'pointed to' by an element in $A$
$$
b \in B \text{ there is a } a \in A \text{ for which } f(a)=b
$$
### Injectivity
A function is injective (or 1:1) if whenever $f(a_1) = f(a_2)$ then $a_1 = a_2$
- i.e. elements in $A$ only 'point' to one element $B$
- i.e. **some** elements in $B$ are pointed to by unique elements in $A$
$$
f(a_1)=f(a_2) \text{ we also have } a_1 = a_2
$$
A function is **bijective** whenever both conditions hold true.
### Function compositions
A composition of two functions $f$ and $g$ (denoted by $f \circ g$) is a function from $D_g$ to $CO_f$ 
- i.e. $f \circ g(x) = f(g(x))$, for all $x \in D_g$
- $x \in D_g$ because $g$ takes the input
- The codomain is given by $f$ since gives the final evaluation
- This also implies that $R_g \subseteq D_f$ as $g$ can only output values valid for $f$
### The identity function*
The function $\text{id}_A \text{ : } A \rightarrow A$ defined by $\text{id}_A(a) = a$, for all $a \in A$ is called the **identity** functions of the set $A$
- i.e. if you plug an arbitrary value $a \in A$ then it will output $a$ again.
- 'y = x'
### Invertibility
A function $f \text{ : } A \rightarrow B$ is invertible $\iff$ there is a function $g \text{ : } B \rightarrow A$ for which $f \circ g = \text{id}_B$ AND $g \circ f = \text{id}_A$. If there conditions are fulfilled, then $g$ is an inverse of $f$, denoted by $f^{-1}$ 
i.e. there is a $f^{-1} \iff$
$$
f^{-1} \text{ : } B \rightarrow A
$$
$$
f \circ g = \text{id}_B \space\space \text{ AND } \space \space g \circ f = \text{id}_A
$$
***
### Example
let $f \text{ : } \{1,2,3\} \rightarrow \{1,2\}$ with the rule $f(1) = 1$, $f(2) = 1$, and $f(3) = 2$.

Evaluate whether a function $f^{-1}$ exists.

We need to find a function (for now, lets call it $g$) that fulfills the requirements:
1. $g \text{ : } \{1,2\} \rightarrow \{1,2,3\}$
2. $f \circ g = \text{id}_{\{1,2\}}$ 
3. $g \circ f = \text{id}_{\{1,2,3\}}$ 

For [1], simply let $g \text{ : } \{1,2\} \rightarrow \{1,2,3\}$

For [2], we need to create a rule for $g$ such that  $f \circ g (x) = \text{id}_{\{1,2\}}$ where $x \in D_g$ 
- i.e. $f(g(x)) = x$
Recall how $f(1) = 1$, $f(2) = 1$, and $f(3) = 2$.
Let $g(1) = 1 \wedge g(2) = 2$ and $g(2) = 3$. This way, whenever we do $f(g(x)) \text{ for } x \in D_g$ we always get $x$ back. This fulfills [2]

For [3], we need to, say have a function $h$, (honestly, i don't know why they can be different functions. i think it's just to show that this case in particular is not possible, via contradiction), which fulfills the requirement $g \circ f = \text{id}_{\{1,2, 3}\}$
- i.e. $g \circ f(x) = x$ for $x \in D_f$ where $D_f = {1,2,3}$

Beginning with making it so $h(f(1)) = 1$: Since $f(1) = 1$, we can simply say that $h(1) = 1$
Next, make $h(f(2)) = 1$: Since $f(2) = 1$, we can simply say that $h(1) = 2$ 

IS WHAT I WOULD SAY

but we just said $h(1) = 1$; we can't re-assign the value of $h(1)$ and say it to be equal to two at the same time. That would no longer be a function.

Thus, it is demonstrated that condition [3] CANNOT be fulfilled and thus $f$ does **not** have an inverse

***
## 1.8 Images and pre-images
Given a function $f  \text{ : } A \rightarrow B$ , and a subset $S$ of $A$ ($S \subseteq A)$, the image of $S$ under $f$ is the set:
$$
f(S) = \{f(s) \text{ | }  s\in S\}
$$
If $T$ is a subset of $B$ ($T \subseteq B$), then the pre-image (or the inverse image) of $T$ under $f$ is the set given by:
$$
f^{-1}(T)=\{a \in A \text{ | } f(a) \in T\}
$$
Note that the two are sets.
***
### Example 1.4
Let $f \text{ : } A \times B \rightarrow B$ be the projection onto the second component. For every arbitrary element $b \in B$, find the pre-image $\{b\}$ ==**(this is a set)**== under $f$
- i.e. what is the definition of $f^{-1}(\{b\})$ where $b$ is basically $b \in B$ (just think of $b$ as an arbitrary element within $B$)

By the definition of a pre-image (see [1.8]) :
$$
f^{-1}(\{b\}) = \{(x,y) \in A \times B\ \text{ | } f(x,y) \in \{b\}\}
$$
*note how we are asking for two points as $D_f$ is defined as the cartesian product of $A$ and $B$
- i.e. **"The set of points (x,y) within the set created by $A \times B$ such that whenever we apply $f$ to these points we get points within the set $\{b\}$**

Now, by recognizing the fact that the $x$ input does not affect the output of the function, $f$ can be treated as a function which 'spits whatever $y$ is back out, regardless of $x$' i.e.:
$$
f(x,y) \in B \Rightarrow\forall x \in A, f(x, y) = y \in B
$$
Treat $y$ as any arbitrary value $y \in \{b\}$ . Basically all this is saying is that if you, for example, do f(x, 2), then the output will **always** be 2 regardless of x. This is why it can be said that in this case,
$$
\forall x \in A \text{ | } f(x,2) =2
$$
This lets us simplify out original statement ($f^{-1}(\{b\}) = \{(x,y) \in A \times B\ \text{ | } f(x,y) \in \{b\}\}$) to:
$$
f^{-1}(\{b\}) = \{(x,y) \in A \times B\ \text{ | } y \in \{b\}\}
$$
i.e. "given an arbitrary input $y \in \{b\}$, give me EVREY sets such that $y$ IS $y$." And by the definition of the function, this is again every single possible input for the first side (i.e. $\forall x \in A)$ and the arbitrary input y. This translates this
$$
f^{-1}(\{b\}) = \{(x,y) \in A \times B\ \text{ | } y = b\}
$$
$$
f^{-1}(\{b\}) = \forall x \in A, x \times y 
$$
honestly im still kinda confused by whatever
***
### Example 1.5
For $f \text{ : } \mathbb{R}^2 \rightarrow \mathbb{R}$ be a function defined by $f(x,y)=2x+3y$. For $b \in \mathbb{R}$, evaluate and describe $f^{-1}(\{b\})$. How do these pre-images change as x changes?

Refer back to the definition of a pre-image:
$$
f^{-1}(\{b\}) = \{ (x,y) \in \mathbb{R}^2\ \text{| } f(x,y) \in \{b\}\}
$$
We can substitute in the function's definition:
$$
f^{-1}(\{b\}) = \{ (x,y) \in \mathbb{R}^2\ \text{| } 2x+3y \in \{b\}\}
$$
By recognizing that we are not plugging in a whole ass set all at once, and instead just an arbitrary value $b \in \{b\}$ , we can see that all this function really is:
$$
\forall b, f^{-1}(b) = \forall b,\{ (x,y) \in \mathbb{R}^2\ \text{| } 2x+3y \in b\} 
$$
Since $b$ is only one element, we can see that this simplifies to:
$$
\forall b, f^{-1}(b) = \forall b,\{ (x,y) \in \mathbb{R}^2\ \text{| } 2x+3y = b\} 
$$
Suddenly, we see that this is basically just a function that outputs "the set of points $(x,y)$ which when we apply the rule $2x+3y$ to them, are equal to an arbitrary point $b \in {b}$" i.e.
$$
2x+3y = b \in \{b\}
$$
PUTTING THIS INTO MORE UNDERSTABLE FORM:
$\{b\} \subseteq \mathbb{R}$, lets say $\{1,\rightarrow,10\}$. Please see [this](https://www.desmos.com/calculator/tzje70phgg)

IT'S JUST A LINE FORMED BY $2x+3y = b$. The line represents the set of all $(x,y)$ that fulfill the rule. THAT'S IT.

doing some algebra, we can see that this is a line
$$
y=\frac{b}{3}-\frac{2}{3}x
$$
'a line with slope $-\frac{2}{3}$ and y-intercept $\frac{b}{3}$'.

In a similar manner, without going into much detail, the inverse of $f^{-1}(z)=\sqrt{x^2 + y^2}$ is just a circle of radius $z$ that represents the set of all values $(x,y)$ that are at a distance $z$ from the origin.
The image would be an arbitrary set $\{z\} \in \mathbb{R}$. it'd just look like a thick circle/donut.
***
## Theorem 1.2 properties of pre-images
Suppose $f \text{ : } A \rightarrow B$ is a function. suppose also that there is a set $S$ such that $S \subseteq A$.  a set $T$ such that $T \subseteq B$ and a set $T_i$ such that $T_i \subseteq B$ for every $i \in I$, where $I$ is a non-empty set. Then:
$$
S \subseteq f^{-1}(f(S)), \text{ and } f(f^{-1}(T)) \subseteq T
$$
$$
f^{-1}(\bigcup\limits_{i \in I} T_i) = \bigcup\limits_{i \in I} f^{-1}(T_i)
$$
$$
f^{-1}(\bigcap\limits_{i \in I} T_1) = \bigcap\limits_{i \in I} f^{-1}(T_1)
$$
### Proof for the first one:
Suppose $s \in S$. By the definition of an image, $f(s) \in f(S)$. Therefore, by the definition of a pre-image $s \in f^{-1}(f(S))$. Thus showing that $S \subseteq f^{-1}(f(S))$