![vid](https://www.youtube.com/watch?v=sW823lmew64&list=PLciPFwfwQdT9QD6P62J6xBbrs2yJFP3RF&index=3)
### Reminders about proofs
1. You cannot prove a universal statement (like, 'for all') by examples. If you are asked to prove 
"The sum of every two odd integers is even" your proof may not be something along the lines of "3 is odd, 5 is odd, and 3+5=8 which is even, thus the sum of all odds is even"

2. Always use distinct variables when referring to different things

3. Only assume was is given in the assumption.

4. All steps must be justified and these justifications must be clearly communicated

5. Only 'known' facts may be utilized. These are definitions, theorems, common axioms etc.

6. To prove a statement in the form "$p$ if and only if q (i.e. $p \iff$ q)", then you must prove both "if $p$ then $q$ (i.e. $p \Rightarrow q$)" AND "if $q$, then $p$ (i.e. $q \Rightarrow p$)"

## 1.3.1 Direct Proofs
In this method, we start w/ the assumption and by taking logical steps we end up with a conclusion.
***
### Example 1.6
Prove that for a function $f \text{ : } \mathbb{R} \rightarrow \mathbb{R}$ defined by the rule $f(x)=x^2+2x$ is one-to-one

By the definition of a 1:1 function (please see [[1.2 Functions]]), show:
$$
f(x)=f(y) \Rightarrow x = y
$$
i.e. Two values $x$ and $y$ can make the function have the same point if and only if $x$ and $y$ are equal (or the same)

So, let's begin with that assumption: $f(x) = f(y)$ for this function $f$. This is equivalent to
$$
x^3+2x=y^3+2y \space\space \text{ or } \space\space x^3-y^3+2(x-y)=0
$$
Which by applying the cubic factoring formula: $a^3 - b^3 = (a-b)(a^2+ab+b^2)$ 
$$
(x-y)(x^2+xy+y^2)2(x-y) = 0 
$$
Which logically gives us two possibilities:
1. $x-y =0$
2. $x^2+xy+y^2 = 0$
Option 1. would imply that $f(x) = f(y) \Rightarrow x=y$. Naturally, this would verify out claim that $f(x) = f(y) \Rightarrow x=y$, but must also check the second possibility, since only one of them has to be correct in order for the entire expression to be zero. There could be a case where option 1 is false but option 2 is not.

Using the quadratic formula, we can try to find a value $x$ such that the whole expression evaluates to is 0 in terms of $y$
$$
x=\frac{-y \pm \sqrt{y^2-4(y^2+2)}}{2}
$$
In this expression we can see that the discriminant (the part inside the root) simplifies to:
$$
-3y^2-8
$$
This expression is **negative** for all $y$, and thus we can't take its root and get a real answer. This implies that there is no such value $x$ so that the expression $x^2+xy+y^2 = 0$ holds true. This means that the second option is **false**, thus leaving us only with option 1. Since this implies that $f(x)=f(y) \Rightarrow x=y$, then the function $f$ is in fact one to one by the definition of a one to one function.
***
## 1.3.2 Proof by contradiction
In this method, we assume the conclusion is false while the assumption is true. After taking logical steps with this assumption in mind, we arrive at a contradiction with the purpose of showing that our initial assumption was false. A **contradiction** is any statement that is false. This could be a violation of a theorem, $1=0$ etc. When using proof by contradiction make sure to specify that this is the method being utilized. Write something along the lines of "On the contrary assume..." or "By way of contradiction, assume" etc.
***
### Example 1.7 
Prove that there are infinitely many primes.

this one is copied straight from the notes cause idfk number theory ok.

On the contrary assume there are only a finite number of primes, and let $p_1, p_2, . . . , p_n$ be the list of all primes. Since the integer $d = p_1 · · · p_n + 1$ is more than one, $d$ has a prime factor. Since $p_1, p_2, . . . , p_n$ is the list of all primes, one of the $p_i$'s must divide $d$. On the other hand $p_i$ divides $p_1p_2 · · · p_n$. Therefore, $p_i$ must divide $d − p_1p_2 · · · p_n = 1$. This is a contradiction. Therefore, the initial assumption must be false, and thus there must exist infinitely many primes.
***
## 1.3.3 [Proof by induction](https://www.youtube.com/watch?v=wblW_M_HVQ8&ab_channel=KhanAcademy)
To prove a statement $P(n)$ (i.e. a statement that depends on a positive integer $n$) engage in the following:

1. Prove $P(1)$ (the basis step) and
2. Assume $P(n)$ holds form some $n \geq 1$, and then prove $P(n+1)$ (inductive step).

i.e. show that a base case is true and then show that a general case $n+1$ is true. Since $P(1)$ is true, then that would imply that $P(2)$ is true since $2 = 1+1$. But then this would also imply $P(3)$ and so on.

If you need to use $P(n-1)$ in your proof of $P(n+1)$, the the basis step must involve two consecutive integers such as $P(1)$ and $P(2)$ and so on. I.e. if your proof relies on two consecutive $n$s, then the basis step needs to show that it is valid for two consecutive $n$.

Often times an alternative **strong induction** is utilized. This involves assuming that $P(n)$ is true for all $n$ leading up to an integer $k$ i.e. Assume that $P(1), P(2), ... P(k)$ holds true.

Always communicate when you are using induction; something along the lines of "We will prove *statement* by induction on *variable*." Also, clearly separate the basis and inductive steps.
***
### Example from the video
Let a function $S(n)$ be the sum of all positive integers leading to $n$, including $n$:
$$
S(3)=1+2+3=6 \space\space \text{ and } \space\space S(4)=1+2+3+4=10
$$
Prove that $S(n)=\frac{n(n+1)}{2}$ using induction

First prove the base case $n=1$. In this case:
$$
S(1)=\frac{1(1+1)}{2}=\frac{2}{2}=1
$$
Since we have shown that this base case is true, we can assume that for some $k$:$$
S(k)=\frac{k(k+1)}{2}
$$(we can do this because we showed that it is true for $k=1$, so technically it is true for *some* $k$)
Now, lets consider the input $k+1$ into $S(k+1)$. This looks something like:
$$
S(k+1)=1+2+3+...+k+k+1
$$
Now, we know that $1+2+3+...+k$ is in fact $\frac{k(k+1)}{2}$ via out assumption. Thus, we can rewrite $S(k+1)$ as:
$$
S(k+1)=\frac{k(k+1)}{2}+k+1=\frac{k(k+1)}{2}+\frac{2(k+1)}{2}=\frac{k(k+1)+2(k+1)}{2}
$$
$$
\Rightarrow \frac{(k+1)(k+2)}{2}=\frac{(k+1)((k+1)+1)}{2}
$$
And this statement right here shows that $S(k+1)$ is equivalent to our defined $S(k+1)$. (outside parentheses k+1 and inside parentheses k+1).

We showed that by assuming $S(k)=\frac{k(k+1)}{2}$, then the expression $\frac{(k+1)(k+1 + 1)}{2}$ is equivalent to $S(k+1)$. I that's as clearly as I can put it. if confused check video and through steps.

Conclusion: By showing that $S(1)$ is true, when we were able to assume that $S(k)$ is true for some value $k$. With this assumption, we found that the statement $S(k+1)$ abides by our assumed rule, thus proving that $S(k+1)$ is equivalent to our assumption expression + 1. Since $k$ is an arbitrary value, and we proved $k = 1$, then by induction this is proven for all integers.
***
